rope ops

rope.fst
@@ -8,6 +8,7 @@ type tree =
     | Leaf : (str:string) -> (sweight:nat{String.strlen str = sweight}) -> tree
     | Node : left:tree -> nweight:nat -> right:tree -> tree
 
+// Add some specs or Lemmas about this
 val str_of_rope: a:tree -> Tot string
 let rec str_of_rope a = match a with
   | Leaf s w -> s
@@ -23,10 +24,22 @@ let get_left a = match a with
   | Node l _ _ -> l
   | _ -> a
 
-val is_rope: a:tree -> Tot (b:bool {b = true <==> (get_weight a = String.length (str_of_rope (get_left a)))})
-let is_rope a = get_weight a = String.length (str_of_rope (get_left a))
+val get_right: a:tree -> Tot (t:tree{(Leaf? a ==> t = a) /\ (Node? a ==> (exists l w. a = Node l w t))})
+let get_right a = match a with
+  | Node _ _ r -> r
+  | _ -> a
+
+val is_rope: a:tree -> Tot bool
+let rec is_rope a = match a with
+| Leaf s w -> w = String.length s
+| Node l w r -> w = String.length (str_of_rope l) && is_rope l && is_rope r
 
 type rope = a:tree{is_rope a}
+
+
+val is_rope': a:rope -> Lemma (requires True) (ensures (get_weight a = String.length (str_of_rope (get_left a)) /\
+                                                    (Node? a ==> is_rope (get_left a) /\ is_rope (get_right a)))) [SMTPat (is_rope a)]
+let is_rope' a = ()
 
 let _ = assert(is_rope (Node (Leaf (String.make 3 (Char.char_of_int 2)) 3) 3 (Leaf (String.make 1 (Char.char_of_int 3)) 1)))
 
@@ -35,7 +48,15 @@ let _ = assert(is_rope (Node (Leaf (String.make 3 (Char.char_of_int 2)) 3) 4 (Le
 
 val get: r:rope -> i:nat{i < String.length (str_of_rope r)} -> Tot (c:String.char{String.index (str_of_rope r) i = c})
 
-let get r i = admit(); Char.char_of_int 5
+#set-options "--initial_fuel 5 --ifuel 5 --initial_ifuel 5 --fuel 5 --z3rlimit 10000"
+
+let rec get tr i = match tr with
+    | Leaf s w -> String.index s i
+    | Node l w r -> assert(i < w ==> String.length (str_of_rope l) >= i);
+                   assert(i >= w ==> String.length (str_of_rope l) <= i);
+                   assert(i < w ==> (exists c. String.index (str_of_rope l) i = c));
+                   // assert(i >= w ==> (exists c. String.index (str_of_rope r) (i-w) = c));
+                   if i < w then (admit(); get l i) else (admit(); get r (i-w))
 
 val set: r:rope -> c:String.char -> i:nat{i < String.length (str_of_rope r)} ->
                 Tot (res:rope{String.length (str_of_rope r) = String.length (str_of_rope res) /\
@@ -50,6 +71,7 @@ val concat: r1:rope -> r2:rope -> Tot (r:rope{str_of_rope r = String.concat "" [
 
 val insert: r:rope -> i:nat{i < String.length (str_of_rope r)} -> s:string ->
                    Tot (res:rope{str_of_rope res = String.concat "" [str_of_rope (fst (split r i)) ; s ; str_of_rope (snd (split r i))]})
+
 
 val delete: r:rope -> i:nat{i < String.length (str_of_rope r)} -> j:nat{i < j /\ j < String.length (str_of_rope r)}
             -> Tot (res:rope{str_of_rope res = String.concat "" [str_of_rope (fst (split r i)); str_of_rope (snd (split r j))]})
